Add FMA's to word and data lang and start fixing broken proofs

compiler/backend/semantics/wordPropsScript.sml
@@ -2480,10 +2480,10 @@ val inst_ok_less_def = Define`
     (c.two_reg_arith ==> (d1 = d2)) ∧
     fp_reg_ok d1 c  ∧ fp_reg_ok d2 c  ∧ fp_reg_ok d3 c) ∧
   (inst_ok_less c (FP (FPFma d1 d2 d3 d4)) <=>
-      (* FIXME: c.two_reg_arith ?? *)
+    2 < c.fp_reg_count /\
     fp_reg_ok d1 c /\ fp_reg_ok d2 c /\ fp_reg_ok d3 c /\ fp_reg_ok d4 c) /\
   (inst_ok_less c (FP (FPFms d1 d2 d3 d4)) <=>
-      (* FIXME: c.two_reg_arith ?? *)
+    2 < c.fp_reg_count /\
     fp_reg_ok d1 c /\ fp_reg_ok d2 c /\ fp_reg_ok d3 c /\ fp_reg_ok d4 c) /\
   (inst_ok_less c (FP (FPMov d1 d2)) ⇔ fp_reg_ok d1 c  ∧ fp_reg_ok d2 c) ∧
   (inst_ok_less c (FP (FPMovToReg r1 r2 d)) ⇔
