compiler/backend/data_liveScript.sml
@@ -39,6 +39,7 @@ val is_pure_def = Define `
   (is_pure (WordFromWord b) = F) /\
   (is_pure (FP_uop _) = F) /\
   (is_pure (FP_bop _) = F) /\
+  (is_pure (FP_top _) = F) /\
   (is_pure ConfigGC = F) /\
   (is_pure _ = T)`
 
@@ -75,6 +76,7 @@ val is_pure_pmatch = Q.store_thm("is_pure_pmatch",`!op.
     | WordFromWord b => F
     | FP_uop _ => F
     | FP_bop _ => F
+    | FP_top _ => F
     | ConfigGC => F
     | _ => T`,
   rpt strip_tac
